Setlec/TTVerify.lean
@@ -41,6 +41,7 @@ import Setlec.TTVerify.OfReduceKey
 import Setlec.TTVerify.SubstConst
 import Setlec.TTVerify.StdAxiomKey
 import Setlec.TTVerify.NatOpPin
+import Setlec.TTVerify.DivModPin
 
 /-!
 # The TTVerify bridge (task #119)
